**5.**
①
$$
\frac{\partial E}{\partial w_5}
= \frac{\partial E}{\partial o} \cdot \frac{\partial o}{\partial w_5}
= (o - 1)h_1
$$

②
$$
\frac{\partial E}{\partial w_6}
= \frac{\partial E}{\partial o} \cdot \frac{\partial o}{\partial w_6}
= (o - 1)h_2
$$

③
$$
\frac{\partial E}{\partial w_1}
= \frac{\partial E}{\partial o} \cdot \frac{\partial o}{\partial h_1} \cdot \frac{\partial h_1}{\partial w_1}
= (o - 1)w_5 \cdot 2
$$

④
$$
\frac{\partial E}{\partial w_2}
= \frac{\partial E}{\partial o} \cdot \frac{\partial o}{\partial h_1} \cdot \frac{\partial h_1}{\partial w_2}
= (o - 1)w_5 \cdot 2
$$

⑤
$$
\frac{\partial E}{\partial w_3}
= \frac{\partial E}{\partial o} \cdot \frac{\partial o}{\partial h_2} \cdot \frac{\partial h_2}{\partial w_3}
= (o - 1)w_6 \cdot 2
$$

**7.**
①
$$
f'(x) = b + \frac{1}{2}(Ax + x^\top A)
$$

②
$$
f'(x) = b + Ax
$$

③
$$
f'(x) = b + (Ax + x^\top A)
$$

④
$$
f'(x) = b
$$

**8.**
①
$$
f''(x) = b^\top + \frac{1}{2}(Ax + x^\top A)
$$

②
$$
f''(x) = 2A
$$

③
$$
f''(x) = 0
$$

④
$$
f''(x) = A
$$

**9.**
①
$$
1 - S(x)
$$

②
$$
S(x')
$$

③
$$
1 - S(x')
$$

④
$$
x
$$

**10.**
①
$$
\begin{pmatrix}
\frac{1}{\sqrt{2}} & \frac{-1}{\sqrt{2}} \\
\frac{-1}{\sqrt{2}} & \frac{1}{\sqrt{2}}
\end{pmatrix}
$$

②
$$
\begin{pmatrix}
0 & 1 \\
1 & 0
\end{pmatrix}
$$

③
$$
\begin{pmatrix}
\cos\theta & -\sin\theta \\
\sin\theta & \cos\theta
\end{pmatrix}
$$

④
$$
\begin{pmatrix}
0 & 0 & 1 \\
1 & 0 & 0 \\
0 & 0 & 1
\end{pmatrix}
$$

⑤ 모두 직교행렬이다.